Added an ARM instruction parser, which removes the need for the GNU assembler. Also added a series of decoding theorems e.g.
|- DECODE_BRANCH (enc (B cond offset)) = (F, offset)

where enc encodes the instruction as a 32-bit word.  This means that
evaluation can occur without the generation of machine code.  The evaluation
speed-up (about 2x) is more modest than I had hoped.  Also, be patient when
building simTheory - these decoding theorems take a while to get through!

More importantly, the decoding theorems make it possible to reason about
ARM instructions, instead of working with machine code.

examples/arm6/evaluate/Data.sml
@@ -1,0 +1,51 @@
+open HolKernel boolLib Parse bossLib;
+
+datatype shift = LSL | LSR | ASR | ROR;
+
+datatype condition = EQ | NE | CS | CC | MI | PL | VS | VC
+                   | HI | LS | GE | LT | GT | LE | AL | NV;
+
+datatype register = R0 | R1 | R2  | R3  | R4  | R5  | R6  | R7
+                  | R8 | R9 | R10 | R11 | R12 | R13 | R14 | R15;
+
+datatype opcode = AND | EOR | SUB | RSB | ADD | ADC | SBC | RSC
+                | TST | TEQ | CMP | CMN | ORR | MOV | BIC | MVN;
+
+datatype addr_mode1 =
+   DpImmediate of num
+ | DpShiftImmediate of {Imm : int, Rm : register, Sh : shift}
+ | DpShiftRegister of {Rm : register, Rs : register, Sh : shift};
+
+datatype addr_mode2 =
+   DtImmediate of int
+ | DtShiftImmediate of {Imm : int, Rm : register, Sh : shift};
+
+datatype msr_mode = MsrImmediate of num | MsrRegister of register;
+
+datatype ARM_instruction =
+    Br of {L : bool, offset : int}
+  | Swi_ex
+  | Data_proc of {opc : opcode, S : bool, Rn : register, Rd : register,
+                  op2 : addr_mode1}
+  | Mla_mul of {A : bool, S : bool, Rd : register, Rn : register,
+                Rs : register, Rm : register}
+  | Ldr_str of {P : bool, U : bool, B : bool, W : bool, L : bool,
+                Rn : register, Rd : register, offset : addr_mode2}
+  | Ldm_stm of {P : bool, U : bool, S : bool, W : bool, L : bool,
+                Rn : register, list : int}
+  | Swp of {B : bool, Rn : register, Rd : register, Rm : register}
+  | Mrs of {R : bool, Rd : register}
+  | Msr of {R : bool, bit19 : bool, bit16 : bool, Op : msr_mode}
+  | Cdp of {Cop1 : int, CRn : register, CRd : register, CP : int,
+            Cop2 :int, CRm : register}
+  | Mcr_mrc of {Cop1 : int, L : bool, Rd : register,
+                CRn : register, CP : int, CRm : register, Cop2 : int}
+  | Ldc_stc of {P : bool, U : bool, N : bool, W : bool, L : bool,
+                CRd : register, Rn : register, CP : int, offset : int}
+  | Undef;
+
+datatype instruction =
+   Instruction of ARM_instruction * condition
+ | Data of num;
+
+exception BadInstruction of string;
