examples/arm6/evaluate/arm_evalLib.sml
@@ -10,20 +10,13 @@ structure arm_evalLib :> arm_evalLib =
 struct
 
 (* interactive use:
-  app load ["Unix", "computeLib", "onestepTheory", "modelsLib",
-            "disassemblerLib", "arm_evalTheory", "instructionTheory"];
+  app load ["computeLib", "onestepTheory", "modelsLib", "arm_evalTheory",
+            "instructionTheory", "instructionSyntax"];
 *)
 
 open HolKernel boolLib bossLib;
 open Parse Q computeLib wordsSyntax rich_listTheory;
-open armTheory arm_evalTheory bsubstTheory;
-
-(* ------------------------------------------------------------------------- *)
-
-val UNDEF_INST  = Arbnum.fromHexString "E6000010";
-val BINUTILS    = "/local/scratch/acjf3/gas/bin/arm-coff-";
-val AS_BIN      = BINUTILS ^ "as";
-val OBJCOPY_BIN = BINUTILS ^ "objcopy";
+open armTheory arm_evalTheory bsubstTheory instructionSyntax;
 
 (* ------------------------------------------------------------------------- *)
 (* Some conversions *)
@@ -55,6 +48,7 @@ val SORT_SUBST_CONV = let open simTheory
          combinTheory.o_THM]
 in
   computeLib.CBV_CONV compset THENC PURE_REWRITE_CONV [Sa_def,Sb_def]
+    THENC SIMP_CONV (srw_ss()) [SUBST_EQ2,simTheory.SUBST_EVAL]
 end;
 
 val SORT_BSUBST_CONV = let open simTheory
@@ -73,8 +67,6 @@ in
   computeLib.CBV_CONV compset THENC SORT_SUBST_CONV
 end;
 
-val SUBST_EQ_CONV = SIMP_CONV (srw_ss()) [SUBST_EQ2,simTheory.SUBST_EVAL];
-
 val ARM_ASSEMBLE_CONV = let open instructionTheory
   val compset = add_rws wordsLib.words_compset
        [transfer_options_accessors,transfer_options_updates_eq_literal,
@@ -85,7 +77,8 @@ val ARM_ASSEMBLE_CONV = let open instructionTheory
         addr_mode2_case_def,msr_mode_case_def,condition_encode_def,
         shift_encode_def,addr_mode1_encode_def,addr_mode2_encode_def,
         msr_mode_encode_def,msr_psr_encode_def,options_encode_def,
-        instruction_encode_def,combinTheory.K_THM]
+        instruction_encode_def,combinTheory.K_THM,
+        SET_NZCV_def,SET_IFMODE_def,mode_num_def,mode_case_def]
 in
   computeLib.CBV_CONV compset
 end;
@@ -96,6 +89,10 @@ fun printn s = print (s ^ "\n");
 
 (* ------------------------------------------------------------------------- *)
 (* Syntax *)
+
+val _ = overload_on("enc", ``instruction_encode``);
+
+fun mk_enc t = mk_comb(``enc``,t);
 
 fun mk_word30 n = mk_n2w(numSyntax.mk_numeral n,``:i30``);
 fun mk_word32 n = mk_n2w(numSyntax.mk_numeral n,``:i32``);
@@ -135,6 +132,16 @@ in
 end;
 
 fun hol_assemble1 m a t = hol_assemble m a [t];
+
+fun assemble m a l = let
+  val code = map ((fn t => if type_of t = ``:word32`` then t else mk_enc t) o
+                  mk_instruction) l
+  val block = listSyntax.mk_list(code,``:word32``)
+in
+  rhsc (SORT_BSUBST_CONV (mk_bsubst(mk_word30 a,block,m)))
+end;
+
+fun assemble1 m a t = assemble m a [t];
 
 (* ------------------------------------------------------------------------- *)
 (* Funtions for memory loading and saving *)
@@ -187,51 +194,6 @@ in
 end;
 
 (* ------------------------------------------------------------------------- *)
-
-(* -----------
- A suitable ARM code binary can be generated using GNU's binutils:
-
-   arm-coff-as -EB assembler.s
-   arm-coff-objcopy -S -j .text a.out code
-
- Then a skip of 60 is needed to pass over the header of the COFF binary
-   ----------- *)
-
-fun assemble m a s =
-  let val as_ex  = Unix.execute(AS_BIN,["-EB","-aln"])
-      val (inp,out) = Unix.streamsOf as_ex
-      val _ = TextIO.output(out,String.concat (map (fn t => t ^ "\n") s))
-      val _ = TextIO.closeOut out
-      val err = TextIO.inputAll inp
-      val _ = TextIO.closeIn inp
-      val args = ["-S","-j",".text","a.out","a.out"]
-      val objcopy_ex = Unix.execute(OBJCOPY_BIN, args)
-      val _ = Unix.reap objcopy_ex
-  in
-    load_mem "a.out" 60 a m handle _ => (printn err; m)
-  end;
-
-fun assemble1 m a s =
-   let val x = if s = "" then UNDEF_INST else Arbnum.fromHexString s in
-      mk_subst(mk_word30 a,mk_word32 x,m)
-   end handle _ => assemble m a [s];
-
-fun disassemble1 m a = disassemblerLib.opcode_string (mem_read m a)
-
-local
-  fun recurse n m a l =
-    if n = 0 then l
-    else recurse (n - 1) m (Arbnum.plus1 a) (disassemble1 m a :: l)
-in
-  fun disassemble n m a = rev (recurse n m a [])
-end;
-
-fun list_mem n m a =
-  let val l = disassemble n m a in
-    (print o String.concat o (map (fn t => t ^ "\n"))) l
-  end;
-
-(* ------------------------------------------------------------------------- *)
 (* Set the general purpose and program status registers *)
 
 val foldl_tm =
@@ -258,13 +220,16 @@ fun init m r s =
    ``STATE_ARMe 0 <| registers := reg; psrs :=  psr;
                      memory := mem; undefined := F |>``;
 
+val STATE_ARMe_NEXT = MATCH_MP onestepTheory.IMAP_NEXT STATE_ARMe_THM;
+
 fun next t =
-  let val t1 = rhsc t
-      val t2 = ((ARMe_CONV THENC ONCE_DEPTH_CONV SORT_BSUBST_CONV
-                   THENC ONCE_DEPTH_CONV SORT_SUBST_CONV
-                   THENC SUBST_EQ_CONV) o
+let val t1 = rhsc t
+    val t2 = ((ARMe_CONV THENC
+                 ONCE_DEPTH_CONV (RAND_CONV (RAND_CONV SORT_BSUBST_CONV)) THENC
+                 ONCE_DEPTH_CONV (RATOR_CONV SORT_SUBST_CONV) THENC
+                 ONCE_DEPTH_CONV (RATOR_CONV (RAND_CONV SORT_SUBST_CONV)) THENC
+                 RATOR_CONV ARM_ASSEMBLE_CONV) o
                  subst [``s:state_arme`` |-> t1]) ``NEXT_ARMe s``
-      val STATE_ARMe_NEXT = MATCH_MP onestepTheory.IMAP_NEXT STATE_ARMe_THM;
   in
      numLib.REDUCE_RULE (MATCH_MP STATE_ARMe_NEXT (CONJ t t2))
   end;
