examples/arm6/evaluate/instructionSyntax.sig
@@ -1,0 +1,27 @@
+signature instructionSyntax =
+sig
+   include Abbrev
+
+   val num_to_arm             : Arbnum.num -> Data.instruction
+   val arm_to_num             : Data.instruction -> Arbnum.num
+   val arm_to_string          : bool -> Data.instruction -> string
+   val string_to_arm          : string -> Data.instruction
+   val arm_to_term            : Data.instruction -> term
+   val term_to_arm            : term -> Data.instruction
+
+   val encode_arm             : string -> Arbnum.num
+   val decode_arm             : Arbnum.num -> string
+   val decode_arm_dec         : string -> string
+   val decode_arm_hex         : string -> string
+
+   val encode_instruction     : term -> Arbnum.num
+   val decode_instruction     : Arbnum.num -> term
+   val decode_instruction_dec : string -> term
+   val decode_instruction_hex : string -> term
+
+   val mk_instruction         : string -> term
+   val dest_instruction       : term -> string
+
+   val pp_instruction         : unit -> unit
+   val remove_pp_instruction  : unit -> unit
+end
