examples/arm6/evaluate/simScript.sml
@@ -7,14 +7,16 @@
 (* ========================================================================= *)
 
 (* interactive use:
-  app load ["onestepTheory", "wordsTheory", "armTheory", "coreTheory",
-            "lemmasTheory", "typesLib", "wordsLib", "bsubstTheory"];
+  app load ["pred_setSimps", "onestepTheory", "wordsTheory", "armLib",
+            "armTheory", "coreTheory", "lemmasTheory", "wordsLib",
+            "bsubstTheory", "instructionTheory", "numeral_bitTheory"];
 *)
 
 open HolKernel boolLib bossLib;
 open Parse Q arithmeticTheory whileTheory bitTheory wordsTheory wordsLib;
 open listTheory rich_listTheory my_listTheory;
 open onestepTheory armTheory coreTheory lemmasTheory bsubstTheory;
+open instructionTheory;
 
 val _ = new_theory "sim";
 
@@ -39,6 +41,9 @@ val word_ss = arith_ss++fcpLib.FCP_ss++wordsLib.SIZES_ss++
 val REDUCE_RULE = numLib.REDUCE_RULE;
 
 (* ------------------------------------------------------------------------- *)
+
+val LESS_THM =
+  CONV_RULE numLib.SUC_TO_NUMERAL_DEFN_CONV prim_recTheory.LESS_THM;
 
 val SUC2NUM = CONV_RULE numLib.SUC_TO_NUMERAL_DEFN_CONV;
 
@@ -176,7 +181,7 @@ val SHIFT_REGISTER_THM = store_thm("SHIFT_REGISTER_THM",
     \\ SIMP_TAC std_ss [SHIFT_REGISTER_def,word_extract_def,
          (GSYM o SIMP_RULE (std_ss++wordsLib.SIZES_ss) [n2w_w2n,BITS_THM,DIV_1,
             (GSYM o SIMP_RULE std_ss [] o SPEC `8`) MOD_2EXP_def] o
-          SPECL [`7`,`0`,`w2n (a:word32)`] o 
+          SPECL [`7`,`0`,`w2n (a:word32)`] o
           Thm.INST_TYPE [alpha |-> ``:i32``]) word_bits_n2w]
     \\ SIMP_TAC word_ss []);
 
@@ -209,7 +214,7 @@ val REGISTER_LIST_THM = store_thm("REGISTER_LIST_THM",
 (* ------------------------------------------------------------------------- *)
 
 val DECODE_INST_THM = store_thm("DECODE_INST_THM",
-  `!n. DECODE_INST (n2w n) = 
+  `!n. DECODE_INST (n2w n) =
         let (q0,r4) = DIVMOD_2EXP 1 (DIV_2EXP 4 n) in
         let (q1,r65) = DIVMOD_2EXP 2 q0 in
         let (q2,r7) = DIVMOD_2EXP 1 q1 in
@@ -259,13 +264,10 @@ val DECODE_INST_THM = store_thm("DECODE_INST_THM",
 
 val word_ss = armLib.fcp_ss ++ wordsLib.SIZES_ss ++ ARITH_ss;
 
-val LESS_THM =
-  CONV_RULE numLib.SUC_TO_NUMERAL_DEFN_CONV prim_recTheory.LESS_THM;
-
 val lem = prove(
   `!w:word32 i. i < 5 ==> (((4 >< 0) w) :word5 %% i = w %% i)`,
   RW_TAC word_ss [word_extract_def,word_bits_def,w2w]);
-  
+
 val PSR_CONS = store_thm("PSR_CONS",
    `!w:word32. w =
        let m = DECODE_MODE ((4 >< 0) w) in
@@ -287,21 +289,13 @@ val PSR_CONS = store_thm("PSR_CONS",
         << [
           FULL_SIMP_TAC std_ss [LESS_THM]
             \\ FULL_SIMP_TAC arith_ss [] \\ EVAL_TAC,
-          EVAL_TAC, 
+          EVAL_TAC,
           `~(mode_num m = 0w)`
             by (Cases_on `m` \\ RW_TAC std_ss [mode_num_def] \\ EVAL_TAC)
             \\ POP_ASSUM MP_TAC \\ UNABBREV_TAC `m`
             \\ RW_TAC (word_ss++ARITH_ss)
                  [DECODE_MODE_def,mode_num_def,n2w_def,lem]
             \\ POP_ASSUM MP_TAC \\ ASM_SIMP_TAC word_ss []]]);
-
-val REG_WRITE_PSR = save_thm("REG_WRITE_PSR",
-  SIMP_CONV std_ss [SET_NZCV_def,SET_IFMODE_def]
-  ``REG_WRITE reg mode Rd (SET_NZCV (n,z,c,v) x)``);
-
-val REG_WRITE_PSR2 = save_thm("REG_WRITE_PSR2",
-  SIMP_CONV std_ss [SET_NZCV_def,SET_IFMODE_def]
-  ``REG_WRITE reg mode Rd (SET_NZCV (n,z,c,v) (SET_IFMODE imask fmask m x))``);
 
 val word_modify_PSR = save_thm("word_modify_PSR",
   SIMP_CONV std_ss [SET_NZCV_def,SET_IFMODE_def]
@@ -555,6 +549,873 @@ val BSa_RULE = store_thm("BSa_RULE", tm1,
 
 val BSb_RULE = store_thm("BSb_RULE", tm2,
   METIS_TAC [BSa_def,BSb_def,BSUBST_BSUBST]);
+
+(* ------------------------------------------------------------------------- *)
+
+val decode_opcode_def = Define`
+  decode_opcode i =
+    case i of
+       AND cond s Rd Rn Op2 -> 0w:word4
+    || EOR cond s Rd Rn Op2 -> 1w
+    || SUB cond s Rd Rn Op2 -> 2w
+    || RSB cond s Rd Rn Op2 -> 3w
+    || ADD cond s Rd Rn Op2 -> 4w
+    || ADC cond s Rd Rn Op2 -> 5w
+    || SBC cond s Rd Rn Op2 -> 6w
+    || RSC cond s Rd Rn Op2 -> 7w
+    || TST cond Rn Op2      -> 8w
+    || TEQ cond Rn Op2      -> 9w
+    || CMP cond Rn Op2      -> 10w
+    || CMN cond Rn Op2      -> 11w
+    || ORR cond s Rd Rn Op2 -> 12w
+    || MOV cond s Rd Op2    -> 13w
+    || BIC cond s Rd Rn Op2 -> 14w
+    || MVN cond s Rd Op2    -> 15w
+    || _ -> ARB`;
+
+val DECODE_PSRD_def = Define`
+  (DECODE_PSRD CPSR_c = (F,F,T)) /\ (DECODE_PSRD CPSR_f = (F,T,F)) /\
+  (DECODE_PSRD CPSR_a = (F,T,T)) /\ (DECODE_PSRD SPSR_c = (T,F,T)) /\
+  (DECODE_PSRD SPSR_f = (T,T,F)) /\ (DECODE_PSRD SPSR_a = (T,T,T))`;
+
+val CONDITION_PASSED3_def = Define`
+  CONDITION_PASSED3 (N,Z,C,V) cond =
+    case cond of
+       EQ -> Z
+    || NE -> ~Z
+    || CS -> C
+    || CC -> ~C
+    || MI -> N
+    || PL -> ~N
+    || VS -> V
+    || VC -> ~V
+    || HI -> C /\ ~Z
+    || LS -> ~C \/ Z
+    || GE -> N = V
+    || LT -> ~(N = V)
+    || GT -> ~Z /\ (N = V)
+    || LE -> Z \/ ~(N = V)
+    || AL -> T
+    || NV -> F`;
+
+val _ = overload_on("enc", ``instruction_encode``);
+
+fun Cases_on_nzcv tm = FULL_STRUCT_CASES_TAC (SPEC tm (armLib.tupleCases
+  ``(n,z,c,v):bool#bool#bool#bool``));
+
+val word_index = METIS_PROVE [word_index_n2w]
+  ``!i n. i < dimindex (UNIV:'a->bool) ==>
+       (((n2w n):bool ** 'a) %% i = BIT i n)``;
+
+val fcp_ss = arith_ss++fcpLib.FCP_ss++wordsLib.SIZES_ss;
+
+val word2_bits = map (fn i => CONJ (EVAL ``BIT 0 ^i``) (EVAL ``BIT 1 ^i``))
+  [``0``,``1``,``2``,``3``];
+
+val BIT_NUMERAL = CONJ (SPECL [`0`,`NUMERAL n`] BIT_def)
+                       (SPECL [`NUMERAL b`,`NUMERAL n`] BIT_def);
+
+fun BIT_CASE_TAC t = POP_ASSUM (SPEC_THEN t
+    (STRIP_ASSUME_TAC o SIMP_RULE fcp_ss [BIT_NUMERAL,BITS_THM]));
+
+val decode_enc_lem = prove(
+  `(!w:word32. (((27 -- 26) w = 0w) = ~(w %% 27) /\ ~(w %% 26))) /\
+   (!w:word32. (((27 -- 26) w = 1w) = ~(w %% 27) /\ (w %% 26))) /\
+   (!w:word32. (((27 -- 26) w = 2w) = (w %% 27) /\ ~(w %% 26))) /\
+   (!w:word32. (((27 -- 26) w = 3w) = (w %% 27) /\ (w %% 26)))`,
+  REPEAT STRIP_TAC \\ Cases_on_word `w`
+    \\ SIMP_TAC fcp_ss [word_bits_def,n2w_def,BIT_ZERO,
+          DECIDE ``(i + 26 <= 27 /\ i + 26 <= 31) = (i = 0) \/ (i = 1)``]
+    \\ (EQ_TAC \\ RW_TAC arith_ss []
+    << [BIT_CASE_TAC `1`,BIT_CASE_TAC `0`,
+     STRIP_ASSUME_TAC (DECIDE ``(i = 0) \/ (i = 1) \/ (2 <= i)``)
+       \\ FULL_SIMP_TAC fcp_ss word2_bits
+       \\ IMP_RES_TAC TWOEXP_MONO2
+       \\ FULL_SIMP_TAC arith_ss [BIT_def,BITS_THM,SUC_SUB,LESS_DIV_EQ_ZERO]]));
+
+val decode_enc_lem2 = prove(
+  `!w:word32. ((6 -- 5) w = 0w) = ~(w %% 6) /\ ~(w %% 5)`,
+  REPEAT STRIP_TAC \\ Cases_on_word `w`
+    \\ SIMP_TAC fcp_ss [word_bits_def,n2w_def,BIT_ZERO,
+          DECIDE ``(i + 5 <= 6 /\ i + 5 <= 31) = (i = 0) \/ (i = 1)``]
+    \\ EQ_TAC \\ RW_TAC arith_ss []
+    << [BIT_CASE_TAC `1`,BIT_CASE_TAC `0`,
+     STRIP_ASSUME_TAC (DECIDE ``(i = 0) \/ (i = 1) \/ (2 <= i)``)
+       \\ FULL_SIMP_TAC fcp_ss word2_bits
+       \\ IMP_RES_TAC TWOEXP_MONO2
+       \\ FULL_SIMP_TAC arith_ss [BIT_def,BITS_THM,SUC_SUB,LESS_DIV_EQ_ZERO]]);
+
+val decode_enc_lem3 = prove(
+  `!w:word32. ((11 -- 5) w = 4w) =
+     ~(w %% 11) /\ ~(w %% 10) /\ ~(w %% 9) /\ ~(w %% 8) /\
+     (w %% 7)  /\ ~(w %% 6)  /\ ~(w %% 5)`,
+  REPEAT STRIP_TAC \\ Cases_on_word `w`
+    \\ SIMP_TAC fcp_ss [word_bits_def,n2w_def,BIT_ZERO,
+         DECIDE ``(i + 5 <= 11 /\ i + 5 <= 31) =
+            (i = 0) \/ (i = 1) \/ (i = 2) \/ (i = 3) \/
+            (i = 4) \/ (i = 5) \/ (i = 6)``]
+    \\ EQ_TAC \\ RW_TAC arith_ss []
+    << [BIT_CASE_TAC `6`,BIT_CASE_TAC `5`,BIT_CASE_TAC `4`,
+        BIT_CASE_TAC `3`,BIT_CASE_TAC `2`,BIT_CASE_TAC `1`,
+        BIT_CASE_TAC `0`,
+     STRIP_ASSUME_TAC (DECIDE ``(i = 0) \/ (i = 1) \/ (i = 2) \/
+          (i = 3) \/ (i = 4) \/ (i = 5) \/ (i = 6) \/ (7 <= i)``)
+       \\ FULL_SIMP_TAC fcp_ss [BIT_NUMERAL,BITS_THM]
+       \\ IMP_RES_TAC TWOEXP_MONO2
+       \\ FULL_SIMP_TAC arith_ss [BIT_def,BITS_THM,SUC_SUB,LESS_DIV_EQ_ZERO]]);
+
+val condition_encode_lem = prove(
+  `!cond i. i < 28 ==> ~(condition_encode cond %% i)`,
+  SIMP_TAC (arith_ss++fcpLib.FCP_ss++wordsLib.SIZES_ss)
+    [condition_encode_def,word_index,w2w,word_lsl_def]);
+
+fun b_of_b t = (GEN_ALL o SIMP_RULE std_ss [BITS_THM] o
+  SPECL [`6`,`0`,`x`,t]) BIT_OF_BITS_THM2;
+
+val shift_encode_lem = prove(
+  `!r. (!i. 6 < i /\ i < 32 ==> ~(shift_encode r %% i)) /\
+       ~(shift_encode r %% 4)`,
+  Cases \\ SIMP_TAC (arith_ss++fcpLib.FCP_ss++wordsLib.SIZES_ss)
+    [shift_encode_def,word_index,w2w,word_or_def,
+     b_of_b `32`, b_of_b `64`, b_of_b `96`] \\ EVAL_TAC);
+
+val DECODE_INST =
+  SIMP_RULE std_ss [decode_enc_lem,decode_enc_lem2,decode_enc_lem3]
+    DECODE_INST_def;
+
+val INDEX_RAND =
+ (GEN_ALL o SIMP_RULE bool_ss [] o ISPEC `\x:word32. x %% i`) COND_RAND;
+
+val BITS_NUMERAL = (GEN_ALL o SPECL [`h`,`l`,`NUMERAL n`]) BITS_def;
+
+val BITS_NUMERAL_ss = rewrites
+  [BITS_NUMERAL,BITS_ZERO2,numeralTheory.numeral_suc,numeralTheory.iDUB_removal,
+   numeral_bitTheory.NUMERAL_DIV_2EXP,numeral_bitTheory.NUMERAL_MOD_2EXP,
+   numeral_bitTheory.iMOD_2EXP,numeral_bitTheory.NUMERAL_DIV2,DIV2_def,NORM_0];
+
+val word_ss = srw_ss()++fcpLib.FCP_ss++wordsLib.SIZES_ss++BITS_NUMERAL_ss++
+  rewrites [INDEX_RAND,BIT_def,word_or_def,word_index,w2w,word_lsl_def,
+    DECODE_INST,condition_encode_lem,instruction_encode_def,shift_encode_lem];
+
+(* ......................................................................... *)
+
+val decode_enc_br = store_thm("decode_enc_br",
+  `(!cond offset. DECODE_INST (enc (instruction$B cond offset)) = br) /\
+   (!cond offset. DECODE_INST (enc (instruction$BL cond offset)) = br)`,
+  RW_TAC word_ss []);
+
+val decode_enc_swi = store_thm("decode_enc_swi",
+  `!cond. DECODE_INST (enc (instruction$SWI cond)) = swi_ex`,
+  RW_TAC word_ss []);
+
+val decode_enc_data_proc = Count.apply prove(
+  `!f. f IN {instruction$AND; instruction$EOR;
+             instruction$SUB; instruction$RSB;
+             instruction$ADD; instruction$ADC;
+             instruction$SBC; instruction$RSC;
+             instruction$ORR; instruction$BIC} ==>
+   (!cond s rd rn r i.
+      DECODE_INST (enc (f cond s rd rn (Dp_immediate r i))) = data_proc) /\
+   (!cond s rd rn sh i.
+      DECODE_INST (enc (f cond s rd rn (Dp_shift_immediate sh i))) =
+        data_proc)`,
+  RW_TAC (std_ss++pred_setSimps.PRED_SET_ss) []
+    \\ RW_TAC word_ss [addr_mode1_encode_def]);
+
+val decode_enc_reg_shift = Count.apply prove(
+  `!f cond s rd rn sh r.
+       f IN {instruction$AND; instruction$EOR;
+             instruction$SUB; instruction$RSB;
+             instruction$ADD; instruction$ADC;
+             instruction$SBC; instruction$RSC;
+             instruction$ORR; instruction$BIC} ==>
+    (DECODE_INST (enc (f cond s rd rn (Dp_shift_register sh r))) = reg_shift)`,
+  RW_TAC (std_ss++pred_setSimps.PRED_SET_ss) []
+    \\ RW_TAC word_ss [addr_mode1_encode_def,shift_encode_def]);
+
+val decode_enc_data_proc2 = prove(
+  `!f. f IN {instruction$TST; instruction$TEQ;
+             instruction$CMP; instruction$CMN} ==>
+   (!cond rn r i.
+      DECODE_INST (enc (f cond rn (Dp_immediate r i))) = data_proc) /\
+   (!cond rn sh i.
+      DECODE_INST (enc (f cond rn (Dp_shift_immediate sh i))) = data_proc)`,
+  RW_TAC (std_ss++pred_setSimps.PRED_SET_ss) []
+    \\ RW_TAC word_ss [addr_mode1_encode_def,shift_encode_def]);
+
+val decode_enc_reg_shift2 = prove(
+  `!f cond rn sh r.
+       f IN {instruction$TST; instruction$TEQ;
+             instruction$CMP; instruction$CMN} ==>
+    (DECODE_INST (enc (f cond rn (Dp_shift_register sh r))) = reg_shift)`,
+  RW_TAC (std_ss++pred_setSimps.PRED_SET_ss) []
+    \\ RW_TAC word_ss [DECODE_INST,addr_mode1_encode_def,shift_encode_def]);
+
+val decode_enc_data_proc3 = prove(
+  `!f. f IN {instruction$MOV; instruction$MVN} ==>
+   (!cond s rd r i.
+      DECODE_INST (enc (f cond s rd (Dp_immediate r i))) = data_proc) /\
+   (!cond s rd sh i.
+      DECODE_INST (enc (f cond s rd (Dp_shift_immediate sh i))) = data_proc)`,
+  RW_TAC (std_ss++pred_setSimps.PRED_SET_ss) []
+    \\ RW_TAC word_ss [addr_mode1_encode_def,shift_encode_def]);
+
+val decode_enc_reg_shift3 = prove(
+  `!f cond s rd sh r.
+       f IN {instruction$MOV; instruction$MVN} ==>
+    (DECODE_INST (enc (f cond s rd (Dp_shift_register sh r))) = reg_shift)`,
+  RW_TAC (std_ss++pred_setSimps.PRED_SET_ss) []
+    \\ RW_TAC word_ss [addr_mode1_encode_def,shift_encode_def]);
+
+val decode_enc_mla_mul = store_thm("decode_enc_mla_mul",
+  `(!cond s rd rm rs.
+      DECODE_INST (enc (instruction$MUL cond s rd rm rs)) = mla_mul) /\
+   (!cond s rd rm rs rn.
+      DECODE_INST (enc (instruction$MLA cond s rd rm rs rn)) = mla_mul)`,
+  RW_TAC word_ss []);
+
+val decode_enc_ldr_str = store_thm("decode_enc_ldr_str",
+  `(!cond opt rd rn offset.
+      DECODE_INST (enc (instruction$LDR cond opt rd rn offset)) = ldr) /\
+   (!cond opt rd rn offset.
+      DECODE_INST (enc (instruction$STR cond opt rd rn offset)) = str)`,
+  REPEAT STRIP_TAC \\ Cases_on `offset` \\ TRY (Cases_on `s`)
+    \\ RW_TAC word_ss [addr_mode2_encode_def,options_encode_def,
+         shift_encode_def,word_modify_def]);
+
+val decode_enc_ldm_stm = store_thm("decode_enc_ldm_stm",
+  `(!cond opt rn list.
+      DECODE_INST (enc (instruction$LDM cond opt rn list)) = ldm) /\
+   (!cond opt rn list.
+      DECODE_INST (enc (instruction$STM cond opt rn list)) = stm)`,
+  RW_TAC word_ss [options_encode_def,word_modify_def]);
+
+val decode_enc_swp = store_thm("decode_enc_swp",
+  `!cond b rd rm rn. DECODE_INST (enc (instruction$SWP cond b rd rm rn)) = swp`,
+  RW_TAC word_ss []);
+
+val decode_enc_mrs = store_thm("decode_enc_mrs",
+  `!cond r rd. (DECODE_INST (enc (instruction$MRS cond r rd)) = mrs_msr) /\
+               ~(enc (instruction$MRS cond r rd) %% 21)`,
+  RW_TAC word_ss []);
+
+val decode_enc_msr = store_thm("decode_enc_msr",
+  `!cond psrd op.
+      (DECODE_INST (enc (instruction$MSR cond psrd op)) = mrs_msr) /\
+      enc (instruction$MSR cond psrd op) %% 21`,
+  REPEAT STRIP_TAC \\ Cases_on `psrd` \\ Cases_on `op`
+    \\ RW_TAC word_ss [msr_psr_encode_def,msr_mode_encode_def]);
+
+val decode_enc_coproc = store_thm("decode_enc_coproc",
+  `(!cond cpn cop1 crd crn crm cop2.
+      DECODE_INST (enc (instruction$CDP cond cpn cop1 crd crn crm cop2)) =
+      cdp_und) /\
+   (!cond. DECODE_INST (enc (instruction$UND cond)) = cdp_und) /\
+   (!cond cpn cop1 rd crn crm cop2.
+      DECODE_INST (enc (instruction$MRC cond cpn cop1 rd crn crm cop2)) =
+      mrc) /\
+   (!cond cpn cop1 rd crn crm cop2.
+      DECODE_INST (enc (instruction$MCR cond cpn cop1 rd crn crm cop2)) = mcr)`,
+  RW_TAC word_ss []);
+
+(* ......................................................................... *)
+
+val word_ss =
+  srw_ss()++ARITH_ss++fcpLib.FCP_ss++wordsLib.SIZES_ss++BITS_NUMERAL_ss++
+  rewrites [INDEX_RAND,word_or_def,word_index,w2w,word_lsl_def,
+    word_bits_def,word_extract_def,condition_encode_lem,
+    instruction_encode_def,shift_encode_lem,BIT_NUMERAL,BIT_ZERO];
+
+val decode_br_enc = store_thm("decode_br_enc",
+  `(!cond offset.
+      DECODE_BRANCH (enc (instruction$B cond offset)) = (F, offset)) /\
+   (!cond offset.
+      DECODE_BRANCH (enc (instruction$BL cond offset)) = (T, offset))`,
+  RW_TAC word_ss [DECODE_BRANCH_def]
+    \\ ASM_SIMP_TAC bool_ss [BIT_SHIFT_THM3,
+         (SYM o EVAL) ``11 * 2 ** 24``,(SYM o EVAL) ``10 * 2 ** 24``]);
+
+val shift_immediate_enc_lem = prove(
+  `(!i r. w2w:word32->word8
+    ((11 -- 7) (w2w (i:word5) << 7 !! w2w (r:word4))) = w2w i) /\
+   (!i r. w2w:word32->word8
+    ((11 -- 7) (w2w (i:word5) << 7 !! 32w !! w2w (r:word4))) = w2w i) /\
+   (!i r. w2w:word32->word8
+    ((11 -- 7) (w2w (i:word5) << 7 !! 64w !! w2w (r:word4))) = w2w i) /\
+   (!i r. w2w:word32->word8
+    ((11 -- 7) (w2w (i:word5) << 7 !! 96w !! w2w (r:word4))) = w2w i) /\
+   (!i r. w2w:word32->word2 ((6 -- 5) (i << 7 !! w2w (r:word4))) = 0w) /\
+   (!i r. w2w:word32->word2 ((6 -- 5) (i << 7 !! 32w !! w2w (r:word4))) = 1w) /\
+   (!i r. w2w:word32->word2 ((6 -- 5) (i << 7 !! 64w !! w2w (r:word4))) = 2w) /\
+   (!i r. w2w:word32->word2 ((6 -- 5) (i << 7 !! 96w !! w2w (r:word4))) = 3w) /\
+   (!i r. w2w:word32->word4 ((3 -- 0) (i << 7 !! w2w (r:word4))) = r) /\
+   (!i r. w2w:word32->word4 ((3 -- 0) (i << 7 !! 32w !! w2w (r:word4))) = r) /\
+   (!i r. w2w:word32->word4 ((3 -- 0) (i << 7 !! 64w !! w2w (r:word4))) = r) /\
+   (!i r. w2w:word32->word4 ((3 -- 0) (i << 7 !! 96w !! w2w (r:word4))) = r)`,
+  RW_TAC word_ss [] \\ FULL_SIMP_TAC std_ss [LESS_THM]
+    \\ ASM_SIMP_TAC word_ss []);
+
+val shift_immediate_enc_lem2 = prove(
+  `(!i r. w2w:word32->word8 ((11 -- 7)
+      (33554432w !! w2w (i:word5) << 7 !! w2w (r:word4))) = w2w i) /\
+   (!i r. w2w:word32->word8 ((11 -- 7)
+      (33554432w !! w2w (i:word5) << 7 !! 32w !! w2w (r:word4))) = w2w i) /\
+   (!i r. w2w:word32->word8 ((11 -- 7)
+      (33554432w !! w2w (i:word5) << 7 !! 64w !! w2w (r:word4))) = w2w i) /\
+   (!i r. w2w:word32->word8 ((11 -- 7)
+      (33554432w !! w2w (i:word5) << 7 !! 96w !! w2w (r:word4))) = w2w i) /\
+   (!i r. w2w:word32->word2 ((6 -- 5)
+      (33554432w !! i << 7 !! w2w (r:word4))) = 0w) /\
+   (!i r. w2w:word32->word2 ((6 -- 5)
+      (33554432w !! i << 7 !! 32w !! w2w (r:word4))) = 1w) /\
+   (!i r. w2w:word32->word2 ((6 -- 5)
+      (33554432w !! i << 7 !! 64w !! w2w (r:word4))) = 2w) /\
+   (!i r. w2w:word32->word2 ((6 -- 5)
+      (33554432w !! i << 7 !! 96w !! w2w (r:word4))) = 3w) /\
+   (!i r. w2w:word32->word4 ((3 -- 0)
+      (33554432w !! i << 7 !! w2w (r:word4))) = r) /\
+   (!i r. w2w:word32->word4 ((3 -- 0)
+      (33554432w !! i << 7 !! 32w !! w2w (r:word4))) = r) /\
+   (!i r. w2w:word32->word4 ((3 -- 0)
+      (33554432w !! i << 7 !! 64w !! w2w (r:word4))) = r) /\
+   (!i r. w2w:word32->word4 ((3 -- 0)
+      (33554432w !! i << 7 !! 96w !! w2w (r:word4))) = r)`,
+  RW_TAC word_ss [] \\ FULL_SIMP_TAC std_ss [LESS_THM]
+    \\ ASM_SIMP_TAC word_ss []);
+
+val shift_register_enc_lem = prove(
+  `(!i r. w2w:word32->word4 ((11 -- 8)
+      (16w !! w2w (i:word4) << 8 !! w2w (r:word4))) = i) /\
+   (!i r. w2w:word32->word4 ((11 -- 8)
+      (16w !! w2w (i:word4) << 8 !! 32w !! w2w (r:word4))) = i) /\
+   (!i r. w2w:word32->word4 ((11 -- 8)
+      (16w !! w2w (i:word4) << 8 !! 64w !! w2w (r:word4))) = i) /\
+   (!i r. w2w:word32->word4 ((11 -- 8)
+      (16w !! w2w (i:word4) << 8 !! 96w !! w2w (r:word4))) = i) /\
+   (!i r. w2w:word32->word2 ((6 -- 5)
+      (16w !! i << 8 !! w2w (r:word4))) = 0w) /\
+   (!i r. w2w:word32->word2 ((6 -- 5)
+      (16w !! i << 8 !! 32w !! w2w (r:word4))) = 1w) /\
+   (!i r. w2w:word32->word2 ((6 -- 5)
+      (16w !! i << 8 !! 64w !! w2w (r:word4))) = 2w) /\
+   (!i r. w2w:word32->word2 ((6 -- 5)
+      (16w !! i << 8 !! 96w !! w2w (r:word4))) = 3w) /\
+   (!i r. w2w:word32->word4 ((3 -- 0)
+      (16w !! i << 8 !! w2w (r:word4))) = r) /\
+   (!i r. w2w:word32->word4 ((3 -- 0)
+      (16w !! i << 8 !! 32w !! w2w (r:word4))) = r) /\
+   (!i r. w2w:word32->word4 ((3 -- 0)
+      (16w !! i << 8 !! 64w !! w2w (r:word4))) = r) /\
+   (!i r. w2w:word32->word4 ((3 -- 0)
+      (16w !! i << 8 !! 96w !! w2w (r:word4))) = r)`,
+  RW_TAC word_ss [] \\ FULL_SIMP_TAC std_ss [LESS_THM]
+    \\ ASM_SIMP_TAC word_ss []);
+
+val immediate_enc = store_thm("immediate_enc",
+  `(!c r i. IMMEDIATE c ((11 >< 0) (addr_mode1_encode (Dp_immediate r i))) =
+      arm$ROR (w2w i) (2w * w2w r) c) /\
+    !c r i. IMMEDIATE c ((11 >< 0) (msr_mode_encode (Msr_immediate r i))) =
+      arm$ROR (w2w i) (2w * w2w r) c`,
+  RW_TAC (word_ss++boolSimps.LET_ss)
+         [IMMEDIATE_def,addr_mode1_encode_def,msr_mode_encode_def]
+    \\ (MATCH_MP_TAC (METIS_PROVE [] ``!a b c d x. (a = b) /\ (c = d) ==>
+         (ROR a c x = ROR b d x)``)
+    \\ STRIP_TAC << [ALL_TAC,
+         MATCH_MP_TAC (PROVE [] ``!a b. (a = b) ==> (2w:word8 * a = 2w * b)``)]
+    \\ RW_TAC word_ss [WORD_EQ]
+    << [Cases_on `i' < 12` \\ ASM_SIMP_TAC word_ss []
+        \\ Cases_on `i' < 8` \\ ASM_SIMP_TAC word_ss [],
+      Cases_on `i' < 4` \\ ASM_SIMP_TAC word_ss []]
+    \\ POP_ASSUM_LIST (ASSUME_TAC o hd)
+    \\ FULL_SIMP_TAC std_ss [LESS_THM]
+    \\ ASM_SIMP_TAC word_ss []));
+
+val immediate_enc2 = store_thm("immediate_enc2",
+  `!i. ((11 >< 0) (addr_mode2_encode (Dt_immediate i))):word12 = i`,
+  RW_TAC word_ss [addr_mode2_encode_def,w2w]
+    \\ Cases_on `i' < 12` \\ ASM_SIMP_TAC word_ss []);
+
+val shift_immediate_enc = store_thm("shift_immediate_enc",
+  `!reg m c sh i. SHIFT_IMMEDIATE reg m c
+      ((11 >< 0) (addr_mode1_encode (Dp_shift_immediate sh i))) =
+      if i = 0w then
+        case sh of
+           LSL Rm -> arm$LSL (REG_READ reg m Rm) 0w c
+        || LSR Rm -> arm$LSR (REG_READ reg m Rm) 32w c
+        || ASR Rm -> arm$ASR (REG_READ reg m Rm) 32w c
+        || ROR Rm -> arm$RRX (REG_READ reg m Rm) c
+      else
+        case sh of
+           LSL Rm -> arm$LSL (REG_READ reg m Rm) (w2w i) c
+        || LSR Rm -> arm$LSR (REG_READ reg m Rm) (w2w i) c
+        || ASR Rm -> arm$ASR (REG_READ reg m Rm) (w2w i) c
+        || ROR Rm -> arm$ROR (REG_READ reg m Rm) (w2w i) c`,
+  REPEAT STRIP_TAC \\ Cases_on `sh`
+    \\ RW_TAC (srw_ss()++wordsLib.SIZES_ss++boolSimps.LET_ss)
+        [SHIFT_IMMEDIATE_def,SHIFT_IMMEDIATE2_def,addr_mode1_encode_def,
+         WORD_BITS_COMP_THM,shift_encode_def,w2w_w2w,word_extract_def,
+         word_bits_w2w,shift_immediate_enc_lem,n2w_11]
+    \\ FULL_SIMP_TAC (std_ss++wordsLib.SIZES_ss)
+        [EVAL ``w2w:word5->word8 0w``,word_0_n2w,w2n_w2w,GSYM w2n_11]);
+
+val shift_immediate_enc2 = store_thm("shift_immediate_enc2",
+  `!reg m c sh i. SHIFT_IMMEDIATE reg m c
+      ((11 >< 0) (addr_mode2_encode (Dt_shift_immediate sh i))) =
+      if i = 0w then
+        case sh of
+           LSL Rm -> arm$LSL (REG_READ reg m Rm) 0w c
+        || LSR Rm -> arm$LSR (REG_READ reg m Rm) 32w c
+        || ASR Rm -> arm$ASR (REG_READ reg m Rm) 32w c
+        || ROR Rm -> arm$RRX (REG_READ reg m Rm) c
+      else
+        case sh of
+           LSL Rm -> arm$LSL (REG_READ reg m Rm) (w2w i) c
+        || LSR Rm -> arm$LSR (REG_READ reg m Rm) (w2w i) c
+        || ASR Rm -> arm$ASR (REG_READ reg m Rm) (w2w i) c
+        || ROR Rm -> arm$ROR (REG_READ reg m Rm) (w2w i) c`,
+  REPEAT STRIP_TAC \\ Cases_on `sh`
+    \\ RW_TAC (srw_ss()++wordsLib.SIZES_ss++boolSimps.LET_ss)
+        [SHIFT_IMMEDIATE_def,SHIFT_IMMEDIATE2_def,addr_mode2_encode_def,
+         WORD_BITS_COMP_THM,shift_encode_def,w2w_w2w,word_extract_def,
+         word_bits_w2w,shift_immediate_enc_lem2,n2w_11]
+    \\ FULL_SIMP_TAC (std_ss++wordsLib.SIZES_ss)
+        [EVAL ``w2w:word5->word8 0w``,word_0_n2w,w2n_w2w,GSYM w2n_11]);
+
+val shift_register_enc = store_thm("shift_register_enc",
+  `!reg m c sh r. SHIFT_REGISTER reg m c
+      ((11 >< 0) (addr_mode1_encode (Dp_shift_register sh r))) =
+      let rs = (7 >< 0) (REG_READ reg m r) in
+        case sh of
+           LSL Rm -> arm$LSL (REG_READ (INC_PC reg) m Rm) rs c
+        || LSR Rm -> arm$LSR (REG_READ (INC_PC reg) m Rm) rs c
+        || ASR Rm -> arm$ASR (REG_READ (INC_PC reg) m Rm) rs c
+        || ROR Rm -> arm$ROR (REG_READ (INC_PC reg) m Rm) rs c`,
+  REPEAT STRIP_TAC \\ Cases_on `sh`
+    \\ RW_TAC (srw_ss()++wordsLib.SIZES_ss++boolSimps.LET_ss)
+        [SHIFT_REGISTER_def,SHIFT_REGISTER2_def,addr_mode1_encode_def,
+         WORD_BITS_COMP_THM,shift_encode_def,w2w_w2w,word_extract_def,
+         word_bits_w2w,shift_register_enc_lem,n2w_11]);
+
+val shift_immediate_shift_register = store_thm("shift_immediate_shift_register",
+  `(!reg m c sh r.
+     ((11 >< 0) (addr_mode1_encode (Dp_shift_register sh r))):word12 %% 4) /\
+   (!reg m c sh i.
+     ~(((11 >< 0) (addr_mode1_encode (Dp_shift_immediate sh i))):word12 %% 4))`,
+  NTAC 6 STRIP_TAC \\ Cases_on `sh` \\ RW_TAC word_ss [addr_mode1_encode_def]);
+
+val decode_data_proc_enc = Count.apply prove(
+  `!f. f IN {instruction$AND; instruction$EOR;
+             instruction$SUB; instruction$RSB;
+             instruction$ADD; instruction$ADC;
+             instruction$SBC; instruction$RSC;
+             instruction$ORR; instruction$BIC} ==>
+   (!cond s rd rn r i.
+      DECODE_DATAP (enc (f cond s rd rn (Dp_immediate r i))) =
+      (T,decode_opcode (f cond s rd rn (Dp_immediate r i)),
+       s,rn,rd,(11 >< 0) (addr_mode1_encode (Dp_immediate r i)))) /\
+   (!cond s rd rn sh i.
+      DECODE_DATAP (enc (f cond s rd rn (Dp_shift_immediate sh i))) =
+      (F,decode_opcode (f cond s rd rn (Dp_shift_immediate sh i)),
+       s,rn,rd,(11 >< 0) (addr_mode1_encode (Dp_shift_immediate sh i)))) /\
+   (!cond s rd rn sh r.
+      DECODE_DATAP (enc (f cond s rd rn (Dp_shift_register sh r))) =
+      (F,decode_opcode (f cond s rd rn (Dp_shift_register sh r)),
+       s,rn,rd,(11 >< 0) (addr_mode1_encode (Dp_shift_register sh r))))`,
+  RW_TAC (std_ss++pred_setSimps.PRED_SET_ss) [decode_opcode_def]
+    \\ SIMP_TAC (srw_ss()) []
+    \\ RW_TAC word_ss [DECODE_DATAP_def,addr_mode1_encode_def]
+    \\ ASM_SIMP_TAC bool_ss [BIT_SHIFT_THM3,(SYM o EVAL) ``256 * 2 ** 12``]
+    \\ FULL_SIMP_TAC std_ss [LESS_THM] \\ ASM_SIMP_TAC word_ss []);
+
+val decode_data_proc_enc2 = Count.apply prove(
+  `!f. f IN {instruction$TST; instruction$TEQ;
+             instruction$CMP; instruction$CMN} ==>
+   (!cond rn r i.
+      DECODE_DATAP (enc (f cond rn (Dp_immediate r i))) =
+      (T,decode_opcode (f cond rn (Dp_immediate r i)),
+       T,rn,0w,(11 >< 0) (addr_mode1_encode (Dp_immediate r i)))) /\
+   (!cond rn sh i.
+      DECODE_DATAP (enc (f cond rn (Dp_shift_immediate sh i))) =
+      (F,decode_opcode (f cond rn (Dp_shift_immediate sh i)),
+       T,rn,0w,(11 >< 0) (addr_mode1_encode (Dp_shift_immediate sh i)))) /\
+   (!cond rn sh r.
+      DECODE_DATAP (enc (f cond rn (Dp_shift_register sh r))) =
+      (F,decode_opcode (f cond rn (Dp_shift_register sh r)),
+       T,rn,0w,(11 >< 0) (addr_mode1_encode (Dp_shift_register sh r))))`,
+  RW_TAC (std_ss++pred_setSimps.PRED_SET_ss) [decode_opcode_def]
+    \\ SIMP_TAC (srw_ss()) []
+    \\ RW_TAC word_ss [DECODE_DATAP_def,addr_mode1_encode_def]
+    \\ ASM_SIMP_TAC bool_ss [BIT_SHIFT_THM3,(SYM o EVAL) ``256 * 2 ** 12``]
+    \\ FULL_SIMP_TAC std_ss [LESS_THM] \\ ASM_SIMP_TAC word_ss []);
+
+val decode_data_proc_enc3 = Count.apply prove(
+  `!f. f IN {instruction$MOV; instruction$MVN} ==>
+   (!cond s rd r i.
+      DECODE_DATAP (enc (f cond s rd (Dp_immediate r i))) =
+      (T,decode_opcode (f cond s rd (Dp_immediate r i)),
+       s,0w,rd,(11 >< 0) (addr_mode1_encode (Dp_immediate r i)))) /\
+   (!cond s rd sh i.
+      DECODE_DATAP (enc (f cond s rd (Dp_shift_immediate sh i))) =
+      (F,decode_opcode (f cond s rd (Dp_shift_immediate sh i)),
+       s,0w,rd,(11 >< 0) (addr_mode1_encode (Dp_shift_immediate sh i)))) /\
+   (!cond s rd sh r.
+      DECODE_DATAP (enc (f cond s rd (Dp_shift_register sh r))) =
+      (F,decode_opcode (f cond s rd (Dp_shift_register sh r)),
+       s,0w,rd,(11 >< 0) (addr_mode1_encode (Dp_shift_register sh r))))`,
+  RW_TAC (std_ss++pred_setSimps.PRED_SET_ss) [decode_opcode_def]
+    \\ SIMP_TAC (srw_ss()) []
+    \\ RW_TAC word_ss [DECODE_DATAP_def,addr_mode1_encode_def]
+    \\ ASM_SIMP_TAC bool_ss [BIT_SHIFT_THM3,(SYM o EVAL) ``256 * 2 ** 12``]
+    \\ FULL_SIMP_TAC std_ss [LESS_THM] \\ ASM_SIMP_TAC word_ss []);
+
+val decode_mla_mul_enc = store_thm("decode_mla_mul_enc",
+  `(!cond s rd rm rs.
+      DECODE_MLA_MUL (enc (instruction$MUL cond s rd rm rs)) =
+      (F,s,rd,0w,rs,rm)) /\
+   (!cond s rd rm rs rn.
+      DECODE_MLA_MUL (enc (instruction$MLA cond s rd rm rs rn)) =
+      (T,s,rd,rn,rs,rm))`,
+  REPEAT STRIP_TAC \\ RW_TAC word_ss [DECODE_MLA_MUL_def]
+    \\ FULL_SIMP_TAC std_ss [LESS_THM] \\ ASM_SIMP_TAC word_ss []);
+
+val decode_ldr_str_enc = Count.apply store_thm("decode_ldr_str_enc",
+  `(!cond opt rd rn i.
+      DECODE_LDR_STR (enc (instruction$LDR cond opt rd rn (Dt_immediate i))) =
+      (F, opt.Pre, opt.Up, opt.BSN, opt.Wb, T, rn, rd,
+       (11 >< 0) (addr_mode2_encode (Dt_immediate i)))) /\
+   (!cond opt rd rn sh i.
+      DECODE_LDR_STR (enc (instruction$LDR cond opt rd rn
+          (Dt_shift_immediate sh i))) =
+      (T, opt.Pre, opt.Up, opt.BSN, opt.Wb, T, rn, rd,
+        (11 >< 0) (addr_mode2_encode (Dt_shift_immediate sh i)))) /\
+   (!cond opt rd rn i.
+      DECODE_LDR_STR (enc (instruction$STR cond opt rd rn (Dt_immediate i))) =
+      (F, opt.Pre, opt.Up, opt.BSN, opt.Wb, F, rn, rd,
+       (11 >< 0) (addr_mode2_encode (Dt_immediate i)))) /\
+   (!cond opt rd rn sh i.
+      DECODE_LDR_STR (enc (instruction$STR cond opt rd rn
+          (Dt_shift_immediate sh i))) =
+      (T, opt.Pre, opt.Up, opt.BSN, opt.Wb, F, rn, rd,
+        (11 >< 0) (addr_mode2_encode (Dt_shift_immediate sh i))))`,
+  REPEAT STRIP_TAC \\ TRY (Cases_on `sh`)
+    \\ RW_TAC word_ss [DECODE_LDR_STR_def,addr_mode2_encode_def,
+         options_encode_def,word_modify_def]
+    \\ FULL_SIMP_TAC std_ss [LESS_THM] \\ ASM_SIMP_TAC word_ss []);
+
+val decode_ldm_stm_enc = store_thm("decode_ldm_stm_enc",
+  `(!cond opt rn l.
+      DECODE_LDM_STM (enc (instruction$LDM cond opt rn l)) =
+      (opt.Pre, opt.Up, opt.BSN, opt.Wb, T, rn, l)) /\
+   (!cond opt rn l.
+      DECODE_LDM_STM (enc (instruction$STM cond opt rn l)) =
+      (opt.Pre, opt.Up, opt.BSN, opt.Wb, F, rn, l))`,
+  RW_TAC word_ss [DECODE_LDM_STM_def,options_encode_def,word_modify_def]
+    \\ FULL_SIMP_TAC std_ss [LESS_THM] \\ ASM_SIMP_TAC word_ss []);
+
+val decode_swp_enc = store_thm("decode_swp_enc",
+  `!cond b rd rm rn.
+      DECODE_SWP (enc (instruction$SWP cond b rd rm rn)) = (b,rn,rd,rm)`,
+  RW_TAC word_ss [DECODE_SWP_def] \\ FULL_SIMP_TAC std_ss [LESS_THM]
+    \\ ASM_SIMP_TAC word_ss []);
+
+val decode_mrs_enc = store_thm("decode_mrs_enc",
+  `!cond r rd. DECODE_MRS (enc (instruction$MRS cond r rd)) = (r, rd)`,
+  RW_TAC word_ss [DECODE_MRS_def]
+    \\ ASM_SIMP_TAC (bool_ss++ARITH_ss) [BIT_SHIFT_THM3,
+         (SYM o EVAL) ``271 * 2 ** 16``,(SYM o EVAL) ``335 * 2 ** 16``]);
+
+val decode_msr_enc = store_thm("decode_msr_enc",
+  `(!cond psrd rot imm.
+      DECODE_MSR (enc (instruction$MSR cond psrd (Msr_immediate rot imm))) =
+        let (r,bit19,bit16) = DECODE_PSRD psrd
+        and opnd = (11 >< 0) (msr_mode_encode (Msr_immediate rot imm)) in
+          (T,r,bit19,bit16,(3 >< 0) opnd,opnd)) /\
+    !cond psrd rm.
+      DECODE_MSR (enc (instruction$MSR cond psrd (Msr_register rm))) =
+        let (r,bit19,bit16) = DECODE_PSRD psrd
+        and opnd = (11 >< 0) (msr_mode_encode (Msr_register rm)) in
+          (F,r,bit19,bit16,rm,opnd)`,
+  REPEAT STRIP_TAC \\ Cases_on `psrd`
+    \\ RW_TAC (word_ss++boolSimps.LET_ss) [DECODE_MSR_def,DECODE_PSRD_def,
+         msr_psr_encode_def,msr_mode_encode_def]
+    \\ ASM_SIMP_TAC (bool_ss++ARITH_ss) [BIT_SHIFT_THM3,
+         (SYM o EVAL) ``4623 * 2 ** 12``, (SYM o EVAL) ``1168 * 2 ** 12``,
+         (SYM o EVAL) ``1152 * 2 ** 12``, (SYM o EVAL) ``1040 * 2 ** 12``,
+         (SYM o EVAL) ``144 * 2 ** 12``, (SYM o EVAL) ``128 * 2 ** 12``,
+         (SYM o EVAL) ``16 * 2 ** 12``]);
+
+val decode_mrc_enc = store_thm("decode_mrc_enc",
+  `!cond cpn cop1 rd crn crm cop2.
+      (15 >< 12) (enc (instruction$MRC cond cpn cop1 rd crn crm cop2)) = rd`,
+  RW_TAC word_ss [] \\ FULL_SIMP_TAC std_ss [LESS_THM]
+    \\ ASM_SIMP_TAC word_ss []);
+
+val decode_ldc_stc_enc = store_thm("decode_ldc_stc_enc",
+  `(!cond opt cpn crd rn offset.
+      DECODE_LDC_STC (enc (instruction$LDC cond opt cpn crd rn offset)) =
+      (opt.Pre, opt.Up, opt.Wb, T, rn, offset)) /\
+   (!cond opt cpn crd rn offset.
+      DECODE_LDC_STC (enc (instruction$STC cond opt cpn crd rn offset)) =
+      (opt.Pre, opt.Up, opt.Wb, F, rn, offset))`,
+  RW_TAC word_ss [DECODE_LDC_STC_def,options_encode_def,word_modify_def]
+    \\ FULL_SIMP_TAC std_ss [LESS_THM] \\ ASM_SIMP_TAC word_ss []);
+
+(* ......................................................................... *)
+
+val BITS_ZERO5 = prove(
+  `!h l n.  n < 2 ** l ==> (BITS h l n = 0)`,
+  RW_TAC arith_ss [BITS_THM,LESS_DIV_EQ_ZERO,ZERO_LT_TWOEXP]);
+
+val BITS_w2n_ZERO = prove(
+  `!w: bool ** 'a. dimindex (UNIV:'a->bool) <= l ==> (BITS h l (w2n w) = 0)`,
+  METIS_TAC [TWOEXP_MONO2,LESS_LESS_EQ_TRANS,BITS_ZERO5,w2n_lt]);
+
+val WORD_BITS_LSL = prove(
+  `!h l n w:bool ** 'a.
+      n <= h /\ n <= l /\ l <= h /\ h < dimindex (UNIV:'a->bool) ==>
+      ((h -- l) (w << n) = ((h - n) -- (l - n)) w)`,
+  RW_TAC (arith_ss++fcpLib.FCP_ss) [WORD_EQ,word_lsl_def,word_bits_def]
+    \\ Cases_on `i + l < dimindex (UNIV:'a->bool)`
+    \\ FULL_SIMP_TAC (arith_ss++fcpLib.FCP_ss) [NOT_LESS_EQUAL,NOT_LESS]);
+
+val condition_code_lem = prove(
+  `!cond. condition_encode cond %% 28 = cond IN {NE;CC;PL;VC;LS;LT;LE;NV}`,
+  Cases \\ RW_TAC (std_ss++wordsLib.SIZES_ss++
+     pred_setSimps.PRED_SET_ss++BITS_NUMERAL_ss)
+   [BIT_def,condition2num_thm,word_rol_def,word_ror_n2w,word_lsl_n2w,
+    w2w_n2w,word_index,condition_encode_def]);
+
+val condition_code_lem2 = prove(
+  `!cond. ~(condition_encode cond %% 28) = cond IN {EQ;CS;MI;VS;HI;GE;GT;AL}`,
+  Cases \\ SIMP_TAC (srw_ss()++pred_setSimps.PRED_SET_ss) [condition_code_lem]);
+
+val condition_code_lem =
+  SIMP_RULE (bool_ss++pred_setSimps.PRED_SET_ss) [] condition_code_lem;
+
+val condition_code_lem2 =
+  SIMP_RULE (bool_ss++pred_setSimps.PRED_SET_ss) [] condition_code_lem2;
+
+val condition_code_lem3 = prove(
+  `!cond. num2condition (w2n ((31 -- 29) (condition_encode cond))) =
+      case cond of
+         EQ -> EQ || NE -> EQ || CS -> CS || CC -> CS
+      || MI -> MI || PL -> MI || VS -> VS || VC -> VS
+      || HI -> HI || LS -> HI || GE -> GE || LT -> GE
+      || GT -> GT || LE -> GT || AL -> AL || NV -> AL`,
+  Cases \\ SIMP_TAC (srw_ss()++wordsLib.SIZES_ss++
+       boolSimps.LET_ss++BITS_NUMERAL_ss)
+    [condition_encode_def,condition2num_thm,num2condition_thm,word_bits_n2w,
+     word_rol_def,word_ror_n2w,word_lsl_n2w,w2w_n2w,w2n_n2w]);
+
+val word_ss = srw_ss()++fcpLib.FCP_ss++wordsLib.SIZES_ss++BITS_NUMERAL_ss++
+  rewrites [word_or_def,word_index,w2w,word_lsl_def,word_bits_def,
+    shift_encode_lem,BIT_def];
+
+val pass_ss =
+ (srw_ss()++ARITH_ss++wordsLib.SIZES_ss++BITS_NUMERAL_ss++boolSimps.LET_ss) ++
+ rewrites [CONDITION_PASSED_def,CONDITION_PASSED2_def,CONDITION_PASSED3_def,
+   GSYM WORD_BITS_OVER_BITWISE,WORD_OR_CLAUSES,BITS_w2n_ZERO,WORD_BITS_LSL,
+   word_bits_n2w,w2w_def,instruction_encode_def,condition_code_lem3];
+
+val condition_addr_mode1 = prove(
+  `(!op2. (31 -- 29) (addr_mode1_encode op2) = 0w) /\
+    !op2. ~((addr_mode1_encode op2) %% 28)`,
+  NTAC 2 STRIP_TAC \\ Cases_on `op2` \\ TRY (Cases_on `s`)
+    \\ RW_TAC pass_ss [addr_mode1_encode_def,shift_encode_def]
+    \\ SIMP_TAC word_ss [BITS_w2n_ZERO]);
+
+val condition_addr_mode2 = prove(
+  `(!op2. (31 -- 29) (addr_mode2_encode op2) = 0w) /\
+    !op2. ~((addr_mode2_encode op2) %% 28)`,
+  NTAC 2 STRIP_TAC \\ Cases_on `op2` \\ TRY (Cases_on `s`)
+    \\ RW_TAC pass_ss [addr_mode2_encode_def,shift_encode_def]
+    \\ SIMP_TAC word_ss [BITS_w2n_ZERO]);
+
+val condition_msr_mode = prove(
+  `(!op2. (31 -- 29) (msr_mode_encode op2) = 0w) /\
+    !op2. ~((msr_mode_encode op2) %% 28)`,
+  NTAC 2 STRIP_TAC \\ Cases_on `op2`
+    \\ RW_TAC pass_ss [msr_mode_encode_def]
+    \\ SIMP_TAC word_ss [BITS_w2n_ZERO]);
+
+val condition_msr_psr = prove(
+  `(!psrd. (31 -- 29) (msr_psr_encode psrd) = 0w) /\
+    !psrd. ~((msr_psr_encode psrd) %% 28)`,
+  NTAC 2 STRIP_TAC \\ Cases_on `psrd`
+    \\ RW_TAC pass_ss [msr_psr_encode_def]
+    \\ SIMP_TAC word_ss []);
+
+val condition_options = prove(
+  `(!opt. (31 -- 29) (options_encode opt) = 0w) /\
+    !opt. ~((options_encode opt) %% 28)`,
+  NTAC 2 STRIP_TAC \\ RW_TAC pass_ss [options_encode_def,word_modify_def]
+    \\ RW_TAC word_ss [] \\ Cases_on `i + 29 < 32`
+    \\ RW_TAC (word_ss++ARITH_ss) []);
+
+val PASS_TAC = REPEAT STRIP_TAC \\ Cases_on_nzcv `flgs`
+  \\ RW_TAC pass_ss [condition_addr_mode1,condition_addr_mode2,
+       condition_msr_mode,condition_msr_psr,condition_options]
+  \\ FULL_SIMP_TAC word_ss [BITS_w2n_ZERO,condition_addr_mode1,
+       condition_addr_mode2,condition_msr_mode,condition_msr_psr,
+       condition_options]
+  \\ RULE_ASSUM_TAC (REWRITE_RULE [condition_code_lem2])
+  \\ FULL_SIMP_TAC (srw_ss()) [condition_code_lem];
+
+(* ......................................................................... *)
+
+val cond_pass_enc_br = store_thm("cond_pass_enc_br",
+  `(!cond flgs offset.
+      CONDITION_PASSED flgs (enc (instruction$B cond offset)) =
+      CONDITION_PASSED3 flgs cond) /\
+   (!cond flgs offset.
+      CONDITION_PASSED flgs (enc (instruction$BL cond offset)) =
+      CONDITION_PASSED3 flgs cond)`,
+  PASS_TAC);
+
+val cond_pass_enc_swi = store_thm("cond_pass_enc_swi",
+  `!cond flgs. CONDITION_PASSED flgs (enc (instruction$SWI cond)) =
+               CONDITION_PASSED3 flgs cond`,
+  PASS_TAC);
+
+val cond_pass_enc_data_proc = prove(
+  `!f. f IN {instruction$AND; instruction$EOR;
+             instruction$SUB; instruction$RSB;
+             instruction$ADD; instruction$ADC;
+             instruction$SBC; instruction$RSC;
+             instruction$ORR; instruction$BIC} ==>
+   (!cond s rd rn op2.
+      CONDITION_PASSED flgs (enc (f cond s rd rn op2)) =
+      CONDITION_PASSED3 flgs cond)`,
+  RW_TAC (std_ss++pred_setSimps.PRED_SET_ss) [] \\ PASS_TAC);
+
+val cond_pass_enc_data_proc2 = prove(
+  `!f. f IN {instruction$TST; instruction$TEQ;
+             instruction$CMP; instruction$CMN} ==>
+   (!cond rn op2.
+      CONDITION_PASSED flgs (enc (f cond rn op2)) =
+      CONDITION_PASSED3 flgs cond)`,
+  RW_TAC (std_ss++pred_setSimps.PRED_SET_ss) [] \\ PASS_TAC);
+
+val cond_pass_enc_data_proc3 = prove(
+  `!f. f IN {instruction$MOV; instruction$MVN} ==>
+   (!cond s rd op2.
+      CONDITION_PASSED flgs (enc (f cond s rd op2)) =
+      CONDITION_PASSED3 flgs cond)`,
+  RW_TAC (std_ss++pred_setSimps.PRED_SET_ss) [] \\ PASS_TAC);
+
+val cond_pass_enc_mla_mul = store_thm("cond_pass_enc_mla_mul",
+  `(!cond s rd rm rs.
+      CONDITION_PASSED flgs (enc (instruction$MUL cond s rd rm rs)) =
+      CONDITION_PASSED3 flgs cond) /\
+   (!cond s rd rm rs rn.
+      CONDITION_PASSED flgs (enc (instruction$MLA cond s rd rm rs rn)) =
+      CONDITION_PASSED3 flgs cond)`,
+  PASS_TAC);
+
+val cond_pass_enc_ldr_str = store_thm("cond_pass_enc_ldr_str",
+  `(!cond opt rd rn offset.
+      CONDITION_PASSED flgs (enc (instruction$LDR cond opt rd rn offset)) =
+      CONDITION_PASSED3 flgs cond) /\
+   (!cond opt rd rn offset.
+      CONDITION_PASSED flgs (enc (instruction$STR cond opt rd rn offset)) =
+      CONDITION_PASSED3 flgs cond)`,
+  PASS_TAC);
+
+val cond_pass_enc_ldm_stm = store_thm("cond_pass_enc_ldm_stm",
+  `(!cond opt rn list.
+      CONDITION_PASSED flgs (enc (instruction$LDM cond opt rn list)) =
+      CONDITION_PASSED3 flgs cond) /\
+   (!cond opt rn list.
+      CONDITION_PASSED flgs (enc (instruction$STM cond opt rn list)) =
+      CONDITION_PASSED3 flgs cond)`,
+  PASS_TAC);
+
+val cond_pass_enc_swp = store_thm("cond_pass_enc_swp",
+  `!cond b rd rm rn.
+      CONDITION_PASSED flgs (enc (instruction$SWP cond b rd rm rn)) =
+      CONDITION_PASSED3 flgs cond`,
+  PASS_TAC);
+
+val cond_pass_enc_mrs = store_thm("cond_pass_enc_mrs",
+  `!cond r rd.
+      CONDITION_PASSED flgs (enc (instruction$MRS cond r rd)) =
+      CONDITION_PASSED3 flgs cond`,
+  PASS_TAC);
+
+val cond_pass_enc_msr = store_thm("cond_pass_enc_msr",
+  `!cond psrd op.
+      CONDITION_PASSED flgs (enc (instruction$MSR cond psrd op)) =
+      CONDITION_PASSED3 flgs cond`,
+  PASS_TAC);
+
+val cond_pass_enc_coproc = store_thm("cond_pass_enc_coproc",
+  `(!cond cpn cop1 crd crn crm cop2.
+      CONDITION_PASSED flgs
+        (enc (instruction$CDP cond cpn cop1 crd crn crm cop2)) =
+      CONDITION_PASSED3 flgs cond) /\
+   (!cond. CONDITION_PASSED flgs (enc (instruction$UND cond)) =
+      CONDITION_PASSED3 flgs cond) /\
+   (!cond cpn cop1 rd crn crm cop2.
+      CONDITION_PASSED flgs
+        (enc (instruction$MRC cond cpn cop1 rd crn crm cop2)) =
+      CONDITION_PASSED3 flgs cond) /\
+   (!cond cpn cop1 rd crn crm cop2.
+      CONDITION_PASSED flgs
+        (enc (instruction$MCR cond cpn cop1 rd crn crm cop2)) =
+      CONDITION_PASSED3 flgs cond)`,
+  PASS_TAC);
+
+(* ......................................................................... *)
+
+fun MAP_SPEC t l = LIST_CONJ (map (fn x =>
+  SIMP_RULE (srw_ss()++pred_setSimps.PRED_SET_ss)
+    [decode_opcode_def] (SPEC x t)) l);
+
+val opc1 =
+ [`instruction$AND`, `instruction$EOR`, `instruction$SUB`, `instruction$RSB`,
+  `instruction$ADD`, `instruction$ADC`, `instruction$SBC`, `instruction$RSC`,
+  `instruction$ORR`, `instruction$BIC`];
+
+val opc2 =
+ [`instruction$TST`, `instruction$TEQ`, `instruction$CMP`, `instruction$CMN`];
+
+val opc3 = [`instruction$MOV`, `instruction$MVN`];
+
+val cond_pass_enc_data_proc = save_thm("cond_pass_enc_data_proc",
+  MAP_SPEC cond_pass_enc_data_proc opc1);
+
+val cond_pass_enc_data_proc2 = save_thm("cond_pass_enc_data_proc2",
+  MAP_SPEC cond_pass_enc_data_proc2 opc2);
+
+val cond_pass_enc_data_proc3 = save_thm("cond_pass_enc_data_proc3",
+  MAP_SPEC cond_pass_enc_data_proc3 opc3);
+
+val decode_data_proc_enc = save_thm("decode_data_proc_enc",
+  MAP_SPEC decode_data_proc_enc opc1);
+
+val decode_data_proc_enc2 = save_thm("decode_data_proc_enc2",
+  MAP_SPEC decode_data_proc_enc2 opc2);
+
+val decode_data_proc_enc3 = save_thm("decode_data_proc_enc3",
+  MAP_SPEC decode_data_proc_enc3 opc3);
+
+val decode_enc_data_proc = save_thm("decode_enc_data_proc",
+  MAP_SPEC decode_enc_data_proc opc1);
+
+val decode_enc_data_proc2 = save_thm("decode_enc_data_proc2",
+  MAP_SPEC decode_enc_data_proc2 opc2);
+
+val decode_enc_data_proc3 = save_thm("decode_enc_data_proc3",
+  MAP_SPEC decode_enc_data_proc3 opc3);
+
+val decode_enc_reg_shift = save_thm("decode_enc_reg_shift",
+  MAP_SPEC decode_enc_reg_shift opc1);
+
+val decode_enc_reg_shift2 = save_thm("decode_enc_reg_shift2",
+  MAP_SPEC decode_enc_reg_shift2 opc2);
+
+val decode_enc_reg_shift3 = save_thm("decode_enc_reg_shift3",
+  MAP_SPEC decode_enc_reg_shift3 opc3);
 
 (* ------------------------------------------------------------------------- *)
 
